APPEND_TRACE_SAME_2_THM uses clocked semantics also

semantics/il2/proofs/il2_compositionScript.sml
@@ -51,34 +51,26 @@ THEN match_mp_tac (GEN_ALL(CONJUNCT2 (SPEC_ALL (REWRITE_RULE [EQ_IMP_THM] RTC_CA
 THEN Q.EXISTS_TAC `SOME (pc, clk, stk, st)` THEN rw []
 THEN match_mp_tac RTC_SUBSET THEN rwa [exec_clocked_one_cases] THEN rwa [fetch_append_thm]);
 
-val incr_pc_def = Define `incr_pc (i, s, stk) (i':int) = (i + i', s, stk)`;
+val incr_pc_def = Define `(incr_pc (SOME (i, clk, s, stk)) (i':int) = SOME (i + i', clk, s, stk)) /\ (incr_pc NONE _ = NONE)`;
 
 val CHANGE_PC_INSTR_THM = store_thm("CHANGE_PC_INSTR_THM",
-``!n x pc s stk pc' s' stk'.exec_instr x (pc, s, stk) (pc', s', stk') <=> exec_instr x (n + pc, s, stk) (n + pc', s', stk')``,
-Cases_on `x` THEN rwa [EQ_IMP_THM, exec_instr_cases] THEN Cases_on `s` THEN fsa [exec_instr_cases] THEN rw[] THEN rwa []);
+``!n x pc clk s stk pc' clk' s' stk'.exec_clocked_instr x (SOME (pc, clk, s, stk)) (SOME (pc', clk', s', stk')) <=> exec_clocked_instr x (SOME (n + pc, clk, s, stk)) (SOME (n + pc', clk', s', stk'))``,
+Cases_on `x` THEN rwa [EQ_IMP_THM, exec_clocked_instr_cases] THEN Cases_on `s` THEN fsa [exec_clocked_instr_cases] THEN rw[] THEN rwa []);
 
 val APPEND_TRACE_SAME_2_THM = store_thm("APPEND_TRACE_SAME_2_THM",
-``!P c c'.exec P c c' ==> !P'.exec (P' ++ P) (incr_pc c (&LENGTH P')) (incr_pc c' (&LENGTH P'))``,
-fs [exec_def] THEN strip_tac
-THEN ho_match_mp_tac RTC_STRONG_INDUCT_RIGHT1 THEN rw [] THEN Cases_on `c` THEN Cases_on `c'` THEN Cases_on `c''` THEN fs [Once exec_one_cases] THEN rw [] THEN fs [incr_pc_def] THEN rw []
+``!P c c'.exec_clocked P c c' ==> !P'.exec_clocked (P' ++ P) (incr_pc c (&LENGTH P')) (incr_pc c' (&LENGTH P'))``,
+fs [exec_clocked_def] THEN strip_tac
+THEN ho_match_mp_tac RTC_STRONG_INDUCT_RIGHT1 THEN rw [] THEN Cases_on `c` THEN Cases_on `c'` THEN Cases_on `c''` THEN fs [Once exec_clocked_one_cases] THEN rw [] THEN fs [incr_pc_def] THEN rw []
+
+THEN (TRY (Cases_on `x` THEN Cases_on `r` THEN Cases_on `r'`)) THEN (TRY (Cases_on `x''` THEN Cases_on `r'` THEN Cases_on `r''`)) THEN (TRY (Cases_on `x'` THEN Cases_on `r'` THEN Cases_on `r''`))
+
+THEN1 (imp_res_tac RTC_CASES1 THEN fs [Once exec_clocked_one_cases, exec_clocked_instr_cases])
 
 
-THEN `exec_instr ((P' ++ P) !! (q' + &LENGTH P')) (&LENGTH P' + q', stk, st) (&LENGTH P' + q'', stk', st')` by (
+THEN1 (Cases_on `P !! pc` THEN fs [Once exec_clocked_instr_cases] THEN rw []
+THEN fs [incr_pc_def] THEN match_mp_tac (GEN_ALL(CONJUNCT2 (SPEC_ALL (REWRITE_RULE [EQ_IMP_THM] RTC_CASES2)))) THEN rw [] THEN Q.EXISTS_TAC `SOME (pc + &LENGTH P', 0, stk, st)` THEN rw [] THEN rwa [exec_clocked_one_cases, exec_clocked_instr_cases, fetch_def, fetch_append_thm, INT_SUB_CALCULATE, INT_ADD_RINV, GSYM INT_ADD_ASSOC])
 
-`P' ++ P !! q' + &LENGTH P' = P !! q'` by (
-
-`0 <= q' + &LENGTH P'` by fsa [int_ge]
-THEN fsa [fetch_append_thm]
-THEN `q' + &LENGTH P' - &LENGTH P' = q'` by fsa []
-THEN metis_tac [])
-
-THEN metis_tac [CHANGE_PC_INSTR_THM])
-
-THEN Cases_on `r` THEN fs [incr_pc_def]
-
-THEN rw [Once RTC_CASES2]
-
-THEN `exec_one (P' ++ P) (q' + &LENGTH P', stk, st) (q'' + &LENGTH P', stk', st')` by rw [exec_one_cases] THEN fsa [] THEN metis_tac [INT_ADD_COMM]);
+THEN match_mp_tac (GEN_ALL(CONJUNCT2 (SPEC_ALL (REWRITE_RULE [EQ_IMP_THM] RTC_CASES2)))) THEN rw [] THEN DISJ2_TAC THEN Q.EXISTS_TAC `SOME (pc + &LENGTH P', clk, stk, st)` THEN rwa [exec_clocked_one_cases] THEN rwa [fetch_append_thm, INT_SUB_CALCULATE, INT_ADD_RINV, GSYM INT_ADD_ASSOC, incr_pc_def] THEN Cases_on `P !! pc` THEN fsa [exec_clocked_instr_cases]);
 
 val EXECUTION_COMPOSE_THM = store_thm("EXECUTION_COMPOSE_THM",
 ``!P P' stk st i' stk' st' i'' stk'' st''.exec P (0, stk, st) (i', stk', st') /\ (&LENGTH P <= i') /\ exec 
